theories/typing/type_context.v
@@ -1,5 +1,9 @@
 From iris.proofmode Require Import tactics.
 From lrust.typing Require Import type lft_contexts.
+From lrust.util Require Import types.
+Require Import Coq.Program.Equality.
+
+
 Set Default Proof Using "Type".
 
 Definition path := expr.
@@ -7,19 +11,18 @@ Bind Scope expr_scope with path.
 
 (* TODO: Consider making this a pair of a path and the rest. We could
    then e.g. formulate tctx_elt_hasty_path more generally. *)
-Inductive tctx_elt `{!typeG Σ} : Type :=
-| TCtx_hasty (p : path) (ty : type)
-| TCtx_blocked (p : path) (κ : lft) (ty : type).
+Inductive tctx_elt `{!typeG Σ} (A : Type) : Type :=
+| TCtx_hasty  (p : path) (ty : type A)
+| TCtx_blocked (p : path) (κ : lft) (ty : type A). 
 
-Notation tctx := (list tctx_elt).
+Notation tctx := (hlist tctx_elt).
 
-Notation "p ◁ ty" := (TCtx_hasty p ty%list%T) (at level 70).
-Notation "p ◁{ κ } ty" := (TCtx_blocked p κ ty)
+Notation "p ◁ ty" := (TCtx_hasty _ p ty%list%T) (at level 70).
+Notation "p ◁{ κ } ty" := (TCtx_blocked _ p κ ty)
    (at level 70, format "p  ◁{ κ }  ty").
 
 Section type_context.
   Context `{!typeG Σ}.
-  Implicit Types T : tctx.
 
   Fixpoint eval_path (p : path) : option val :=
     match p with
@@ -63,19 +66,19 @@ Section type_context.
   Qed.
 
   (** Type context element *)
-  Definition tctx_elt_interp (tid : thread_id) (x : tctx_elt) : iProp Σ :=
+  Definition tctx_elt_interp {A} (tid : thread_id) (x : tctx_elt A) (vπ : proph_asn → A): iProp Σ :=
       match x with
       | p ◁ ty =>
-        ∃ v depth, ⧖depth ∗ ⌜eval_path p = Some v⌝ ∗ ty.(ty_own) depth tid [v]
+        ∃ v depth, ⧖depth ∗ ⌜eval_path p = Some v⌝ ∗ ty.(ty_own) vπ depth tid [v]
       | p ◁{κ} ty => ∃ v, ⌜eval_path p = Some v⌝ ∗
-                  ([†κ] ={⊤}=∗ ∃ depth, ⧖depth ∗ ty.(ty_own) depth tid [v])
+                  ([†κ] ={⊤}=∗ ∃ depth, ⧖depth ∗ ty.(ty_own) vπ depth tid [v])
       end%I.
 
   (* Block tctx_elt_interp from reducing with simpl when x is a constructor. *)
   Global Arguments tctx_elt_interp : simpl never.
 
-  Lemma tctx_hasty_val tid (v : val) ty :
-    tctx_elt_interp tid (v ◁ ty) ⊣⊢ ∃ depth, ⧖depth ∗ ty.(ty_own) depth tid [v].
+  Lemma tctx_hasty_val {A} tid (v : val) (ty : type A) vπ:
+    tctx_elt_interp tid (v ◁ ty) vπ ⊣⊢ ∃ depth, ⧖depth ∗ ty.(ty_own) vπ depth tid [v].
   Proof.
     rewrite /tctx_elt_interp eval_path_of_val. iSplit.
     - iIntros "H". iDestruct "H" as (??) "(#Ht & EQ & ?)".
@@ -83,22 +86,22 @@ Section type_context.
     - iDestruct 1 as (depth) "[??]". eauto.
   Qed.
 
-  Lemma tctx_elt_interp_hasty_path p1 p2 ty tid :
+  Lemma tctx_elt_interp_hasty_path {A} p1 p2 (ty : type A) tid vπ :
     eval_path p1 = eval_path p2 →
-    tctx_elt_interp tid (p1 ◁ ty) ≡ tctx_elt_interp tid (p2 ◁ ty).
+    tctx_elt_interp tid (p1 ◁ ty) vπ ≡ tctx_elt_interp tid (p2 ◁ ty) vπ.
   Proof. intros Hp. rewrite /tctx_elt_interp /=. setoid_rewrite Hp. done. Qed.
 
-  Lemma tctx_hasty_val' tid p (v : val) ty :
+  Lemma tctx_hasty_val' {A} tid p (v : val) (ty : type A) vπ:
     eval_path p = Some v →
-    tctx_elt_interp tid (p ◁ ty) ⊣⊢ ∃ depth, ⧖depth ∗ ty.(ty_own) depth tid [v].
+    tctx_elt_interp tid (p ◁ ty) vπ ⊣⊢ ∃ depth, ⧖depth ∗ ty.(ty_own) vπ depth tid [v].
   Proof.
     intros ?. rewrite -tctx_hasty_val. apply tctx_elt_interp_hasty_path.
     rewrite eval_path_of_val. done.
   Qed.
 
-  Lemma wp_hasty E tid p ty Φ :
-    tctx_elt_interp tid (p ◁ ty) -∗
-    (∀ depth v, ⧖depth -∗ ⌜eval_path p = Some v⌝ -∗ ty.(ty_own) depth tid [v] -∗ Φ v) -∗
+  Lemma wp_hasty {A} E tid p (ty : type A) vπ Φ :
+    tctx_elt_interp tid (p ◁ ty) vπ -∗
+    (∀ depth v, ⧖depth -∗ ⌜eval_path p = Some v⌝ -∗ ty.(ty_own) vπ depth tid [v] -∗ Φ v) -∗
     WP p @ E {{ Φ }}.
   Proof.
     iIntros "Hty HΦ". iDestruct "Hty" as (v depth) "(Hdepth & % & Hown)".
@@ -106,53 +109,79 @@ Section type_context.
     iIntros (v') "%". subst v'. by iApply ("HΦ" with "Hdepth [] Hown").
   Qed.
 
-  Lemma closed_hasty tid p ty : tctx_elt_interp tid (p ◁ ty) -∗ ⌜Closed [] p⌝.
+  Lemma closed_hasty {A} tid p (ty : type A) vπ : tctx_elt_interp tid (p ◁ ty) vπ -∗ ⌜Closed [] p⌝.
   Proof. iDestruct 1 as (??) "(_ & % & _)". eauto using eval_path_closed. Qed.
 
+  (* Fixpoint hzip {F G A B} (x : hlist F A) (y : hlist G B) : hlist (λ ) _. *)
   (** Type context *)
-  Definition tctx_interp (tid : thread_id) (T : tctx) : iProp Σ :=
-    ([∗ list] x ∈ T, tctx_elt_interp tid x)%I.
+  Definition tctx_interp {As} (tid : thread_id) (T : tctx As) (Vs : hlist (λ A, proph_asn → A) As) : iProp Σ :=
+    big_sepHLZip' (λ A x v, tctx_elt_interp tid x v) T Vs.
+  
+  Fixpoint tctx_values {A} π (V : hlist (λ T, proph_asn → T) A) : xprod A :=
+    match V in hlist _ A return xprod A with 
+    | x +:: V => x π -:: tctx_values π V
+    | +[] => -[]
+    end.
 
-  Global Instance tctx_interp_permut tid:
-    Proper ((≡ₚ) ==> (⊣⊢)) (tctx_interp tid).
-  Proof. intros ???. by apply big_opL_permutation. Qed.
+  Lemma tctx_values_distr {T1 T2} (V1 : hlist _ T1) (V2 : hlist _ T2) π : tctx_values π (V1 h++ V2) = tctx_values π V1 -++ tctx_values π V2.
+  Proof. elim V1 => [//| /= ???? -> //]. Qed.
 
-  Lemma tctx_interp_cons tid x T :
-    tctx_interp tid (x :: T) ⊣⊢ (tctx_elt_interp tid x ∗ tctx_interp tid T).
+  Lemma tctx_values_split_l {A B} (V1 : hlist _ A) (V2 : hlist _ B) π : xprod_split_l (tctx_values π (V1 h++ V2)) = tctx_values π V1.
+  Proof. elim/hlist_ind: V1 => [ //| ???? /= -> //=]. Qed.
+
+  Lemma tctx_values_split_r {A B} (V1 : hlist _ A) (V2 : hlist _ B) π : xprod_split_r (tctx_values π (V1 h++ V2)) = tctx_values π V2.
+  Proof. elim/hlist_ind: V1 => [ //| ???? /= -> //=]. Qed.
+
+  Lemma tctx_values_split {A B} (V1 : hlist _ A) (V2 : hlist _ B) π : xprod_split (tctx_values π (V1 h++ V2)) = (tctx_values π V1, tctx_values π V2).
+  Proof. elim/hlist_ind: V1 => [ //| ???? /= -> //=]. Qed.
+
+  Lemma tctx_values_merge {A B} (V1 : hlist _ A) (V2 : hlist _ B) π : tctx_values π V1 -++ tctx_values π V2 = tctx_values π (V1 h++ V2).
+  Proof. elim/hlist_ind: V1 => [ //| ???? /= -> //=]. Qed.
+
+  (* Lemma tctx_interp_permut {As Bs} tid (T1 : tctx As) (T2 : tctx Bs) :
+    T1 ≡ₕₚ T2 -> tctx_interp tid T1  ⊣⊢ tctx_interp tid T2.
+  Proof. apply big_sepHL_permutation. Qed. *)
+
+  Lemma tctx_interp_cons {A As} tid (x : tctx_elt A) (T : tctx As) vπ Vs :
+    tctx_interp tid (x +:: T) (vπ +:: Vs) ⊣⊢ (tctx_elt_interp tid x vπ ∗ tctx_interp tid T Vs).
   Proof. done. Qed.
 
-  Lemma tctx_interp_app tid T1 T2 :
-    tctx_interp tid (T1 ++ T2) ⊣⊢ (tctx_interp tid T1 ∗ tctx_interp tid T2).
-  Proof. rewrite /tctx_interp big_sepL_app //. Qed.
+  Lemma tctx_interp_app {As Bs} tid (T1 : tctx As) V1 (T2 : tctx Bs) V2 :
+    tctx_interp tid (T1 h++ T2) (V1 h++ V2) ⊣⊢ (tctx_interp tid T1 V1 ∗ tctx_interp tid T2 V2).
+  Proof. 
+    induction As as [|?? IH]; dependent destruction T1; dependent destruction V1.
+    - by rewrite left_id.
+    - by rewrite // !tctx_interp_cons -assoc IH.
+  Qed.
 
-  Definition tctx_interp_nil tid :
-    tctx_interp tid [] = True%I := eq_refl _.
+  (* Definition tctx_interp_nil tid :
+    tctx_interp tid +[] = True%I := eq_refl _. *)
 
-  Lemma tctx_interp_singleton tid x :
-    tctx_interp tid [x] ⊣⊢ tctx_elt_interp tid x.
+  Lemma tctx_interp_singleton {A} tid (x : tctx_elt A) v :
+    tctx_interp tid +[x] +[v] ⊣⊢ tctx_elt_interp tid x v.
   Proof. rewrite /tctx_interp /= right_id //. Qed.
 
   (** Copy typing contexts *)
-  Class CopyC (T : tctx) :=
-    copyc_persistent tid : Persistent (tctx_interp tid T).
+  Class CopyC {As: Types} (T : tctx As) Vs :=
+    copyc_persistent tid : Persistent (tctx_interp tid T Vs).
   Global Existing Instances copyc_persistent.
 
-  Global Instance tctx_nil_copy : CopyC [].
+  Global Instance tctx_nil_copy : CopyC +[] +[].
   Proof. rewrite /CopyC. apply _. Qed.
 
-  Global Instance tctx_ty_copy T p ty :
-    CopyC T → Copy ty → CopyC ((p ◁ ty) :: T).
+  Global Instance tctx_ty_copy {A As} (T : tctx As) Vs p (ty : type A) vπ:
+    CopyC T Vs → Copy ty → CopyC  ((p ◁ ty) +:: T) (vπ +:: Vs).
   Proof. intros ???. rewrite tctx_interp_cons. apply _. Qed.
 
   (** Send typing contexts *)
-  Class SendC (T : tctx) :=
-    sendc_change_tid tid1 tid2 : tctx_interp tid1 T -∗ tctx_interp tid2 T.
+  Class SendC {As} (T : tctx As) Vs :=
+    sendc_change_tid tid1 tid2 : tctx_interp tid1 T Vs -∗ tctx_interp tid2 T Vs.
 
-  Global Instance tctx_nil_send : SendC [].
+  Global Instance tctx_nil_send : SendC +[] +[].
   Proof. done. Qed.
 
-  Global Instance tctx_ty_send T p ty :
-    SendC T → Send ty → SendC ((p ◁ ty) :: T).
+  Global Instance tctx_ty_send {A As} (T : tctx As) Vs p (ty : type A) vπ :
+    SendC T Vs → Send ty → SendC ((p ◁ ty) +:: T) (vπ +:: Vs).
   Proof.
     iIntros (HT Hty ??). rewrite !tctx_interp_cons.
     iIntros "[Hty HT]". iSplitR "HT".
@@ -161,126 +190,195 @@ Section type_context.
     - by iApply HT.
   Qed.
 
-  (** Type context inclusion *)
-  Definition tctx_incl (E : elctx) (L : llctx) (T1 T2 : tctx): Prop :=
-    ∀ tid q2, lft_ctx -∗ elctx_interp E -∗ llctx_interp L q2 -∗
-              tctx_interp tid T1 ={⊤}=∗ llctx_interp L q2 ∗ tctx_interp tid T2.
-  Global Instance : ∀ E L, RewriteRelation (tctx_incl E L) := {}.
 
-  Global Instance tctx_incl_preorder E L : PreOrder (tctx_incl E L).
+  (** Type context inclusion *)
+  Definition tctx_incl {A1 A2} (E : elctx) (L : llctx) (T1 : tctx A1) (T2 : tctx A2) (f : (xprod A2 → Prop) → xprod A1 → Prop) : Prop :=
+    ∀ tid q2 V post, lft_ctx -∗ elctx_interp E -∗ llctx_interp L q2 -∗
+              tctx_interp tid T1 V -∗ ⟨ π , f (post π) (tctx_values π V) ⟩ ={⊤}=∗ ∃ V2, llctx_interp L q2 ∗ ⟨ π, post π (tctx_values π V2) ⟩ ∗ tctx_interp tid T2 V2.
+  (* Global Instance : ∀ A E L f, RewriteRelation (@tctx_incl A A E L f) := {}. *)
+
+  (* Global Instance tctx_incl_preorder A E L : PreOrder (@tctx_incl A A E L).
   Proof.
     split.
     - by iIntros (???) "_ _ $ $".
-    - iIntros (??? H1 H2 ??) "#LFT #HE HL H".
+    - rewrite /Transitive. iIntros (??? H1 H2 ??) "#LFT #HE HL H".
       iMod (H1 with "LFT HE HL H") as "(HL & H)".
       by iMod (H2 with "LFT HE HL H") as "($ & $)".
+  Qed. *)
+
+  Lemma tctx_incl_reflexive {A} E L (T : tctx A) : tctx_incl E L T T id. 
+    iIntros (?? V?) "#LFT #HE HL ??".
+    iExists V.
+    by iFrame. 
   Qed.
 
-  Lemma contains_tctx_incl E L T1 T2 : T1 ⊆+ T2 → tctx_incl E L T2 T1.
+
+  Lemma tctx_incl_transitive E L A B C (x : tctx A) (y : tctx B) (z : tctx C) f g :
+    tctx_incl E L x y f → tctx_incl E L y z g → tctx_incl E L x z (f ∘ g).
   Proof.
-    rewrite /tctx_incl. iIntros (Hc ??) "_ _ $ H". by iApply big_sepL_submseteq.
+    iIntros (H1 H2 tid q V post) "#LFT #HE HL H Hp".
+    iMod (H1 with "LFT HE HL H Hp") as (?) "(HL & Hp1 & H)".
+    iMod (H2 with "LFT HE HL H Hp1") as (?) "(? & Hp2 & ?)".
+    iExists V0. by iFrame. 
   Qed.
+(* 
+  Definition xprod_hsubmseteq {As Bs} {T1 : tctx As} {T2 : tctx Bs} (sub : T1 ⊆+ₕ T2) : xprod Bs → xprod As.
+    intros. dependent induction sub; simpl in *; intuition.
+  Qed. *)
 
-  Global Instance tctx_incl_app E L :
-    Proper (tctx_incl E L ==> tctx_incl E L ==> tctx_incl E L) app.
+  (* Lemma contains_tctx_incl {As Bs} E L (T1 : tctx As) (T2 : tctx Bs) (s : T1 ⊆+ₕ T2) : tctx_incl E L T2 T1 (xprod_hsubmseteq s).
   Proof.
-    intros ?? Hincl1 ?? Hincl2 ??. rewrite /tctx_interp !big_sepL_app.
-    iIntros "#LFT #HE HL [H1 H2]".
-    iMod (Hincl1 with "LFT HE HL H1") as "(HL & $)".
-    iApply (Hincl2 with "LFT HE HL H2").
-  Qed.
-  Global Instance tctx_incl_cons E L x :
-    Proper (tctx_incl E L ==> tctx_incl E L) (cons x).
-  Proof. by apply (tctx_incl_app E L [_] [_]). Qed.
+    rewrite /tctx_incl. iIntros (??) "_ _ $ H". by iApply big_sepHL_submseteq.
+  Qed. *)
+  Definition trans_app {A B C D} (f : (Π! A → Prop) → Π! B → Prop) (g : (Π! C → Prop) → Π! D → Prop) : (Π! (A ^++ C) → Prop) → Π! (B ^++ D) → Prop := 
+    λ post bd, f (λ a, g (λ c, post (a -++ c)) (xprod_split_r bd)) (xprod_split_l bd).
 
-  Lemma tctx_incl_frame_l {E L} T T1 T2 :
-    tctx_incl E L T1 T2 → tctx_incl E L (T++T1) (T++T2).
-  Proof. by apply tctx_incl_app. Qed.
-  Lemma tctx_incl_frame_r {E L} T T1 T2 :
-    tctx_incl E L T1 T2 → tctx_incl E L (T1++T) (T2++T).
-  Proof. by intros; apply tctx_incl_app. Qed.
-
-  Lemma copy_tctx_incl E L p `{!Copy ty} :
-    tctx_incl E L [p ◁ ty] [p ◁ ty; p ◁ ty].
-  Proof. iIntros (??) "_ _ $ * [#$ $] //". Qed.
-
-  Lemma copy_elem_of_tctx_incl E L T p `{!Copy ty} :
-    p ◁ ty ∈ T → tctx_incl E L T ((p ◁ ty) :: T).
+  Lemma tctx_incl_app {As Bs Cs Ds} E L (T1 : tctx As) (T1' : tctx Bs) f (T2 : tctx Cs) (T2' : tctx Ds) g:  
+    tctx_incl E L T1 T1' f → tctx_incl E L T2 T2' g → tctx_incl E L (T1 h++ T2) (T1' h++ T2') (trans_app f g).
   Proof.
-    remember (p ◁ ty). induction 1 as [|???? IH]; subst.
-    - apply (tctx_incl_frame_r _ [_] [_;_]), copy_tctx_incl, _.
-    - etrans. by apply (tctx_incl_frame_l [_]), IH, reflexivity.
-      apply contains_tctx_incl, submseteq_swap.
+    intros Hincl1 Hincl2 ????. destruct (hlist_app_split V) as (? & ? & ->). rewrite /tctx_incl /tctx_interp !big_sepHLZip'_app.
+    iIntros "#LFT #HE HL [H1 H2] #HP".
+    iMod (Hincl1 with "LFT HE HL H1 [HP]")  as (W1) "(HL & Hp1 & ?)".
+    { by rewrite /trans_app; setoid_rewrite tctx_values_split_l. }
+    iMod (Hincl2 with "LFT HE HL H2 [Hp1]") as (W2) "(HL & Hp2 & ?)".
+    { by setoid_rewrite tctx_values_split_r. }
+    iExists (W1 h++ W2).
+    rewrite big_sepHLZip'_app.
+    iFrame; by setoid_rewrite tctx_values_distr. 
   Qed.
 
-  Lemma subtype_tctx_incl E L p ty1 ty2 :
-    subtype E L ty1 ty2 → tctx_incl E L [p ◁ ty1] [p ◁ ty2].
+  (* Lemma tctx_incl_frame_l {E L As Bs Cs} (T :tctx As) (T1 : tctx Bs) (T2 : tctx Cs) f:
+    tctx_incl E L T1 T2 f → tctx_incl E L (T +++ T1) (T +++ T2) (xprod_bimap id f).
+  Proof. apply tctx_incl_app, tctx_incl_reflexive. Qed.
+
+  Lemma tctx_incl_frame_r {E L As Bs Cs} (T : tctx As) (T1 : tctx Bs) (T2 : tctx Cs) f :
+    tctx_incl E L T1 T2 f → tctx_incl E L (T1+++T) (T2+++T) (xprod_bimap f id).
+  Proof.  intros. by apply tctx_incl_app, tctx_incl_reflexive. Qed.
+  *)
+
+  Lemma tcx_incl_cons {A As Bs} E L (x : tctx_elt A) (T1 : tctx As) (T2 : tctx Bs) f : 
+    tctx_incl E L T1 T2 f → 
+    tctx_incl E L (x +:: T1) (x +:: T2) (trans_app (id : (Π! ^[A] → Prop) → Π! ^[A] → Prop )  f).
+  Proof.
+    apply (tctx_incl_app E L +[_] +[_]), tctx_incl_reflexive.
+  Qed.
+
+  (*
+  Lemma copy_tctx_incl {A} E L p vπ `{!Copy (ty : type A)} :
+    tctx_incl E L +[p ◁ ty] +[p ◁ ty; p ◁ ty] (λ x, xprod_merge x x).
+  Proof. iIntros (??) "_ _ $ * [#$ $] //". Qed. *)
+
+(* 
+  Lemma copy_elem_of_tctx_incl E L A As (T : tctx As) p `{!Copy (ty : type A)} :
+    p ◁ ty ∈ T → tctx_incl E L T ((p ◁ ty) +:: T).
+  Proof.
+  Qed. *)
+
+  (* Lemma subtype_tctx_incl A B E L (f : A → B) p (ty1 : type A) (ty2 : type B) vπ :
+    subtype E L f ty1 ty2 → tctx_incl E L +[p ◁ ty1] +[p ◁ ty2 [{ f ∘ vπ }]] (xprod_singleton f).
   Proof.
     iIntros (Hst ??) "#LFT #HE HL [H _]".
     iDestruct "H" as (v depth) "(? & % & H)".
     iDestruct (Hst with "HL HE") as "#(_ & _ & Ho & _)". iFrame "HL".
-    iApply big_sepL_singleton. iExists _, _. iFrame "%∗". by iApply "Ho".
-  Qed.
+    iApply big_sepHL_singleton. iExists _, _. 
+    iFrame "%∗". by iApply "Ho".
+  Qed. *)
 
   (* Extracting from a type context. *)
 
-  Definition tctx_extract_hasty E L p ty T T' : Prop :=
-    tctx_incl E L T ((p ◁ ty)::T').
-  Lemma tctx_extract_hasty_further E L p ty T T' x :
-    tctx_extract_hasty E L p ty T T' →
-    tctx_extract_hasty E L p ty (x::T) (x::T').
-  Proof. unfold tctx_extract_hasty=>->. apply contains_tctx_incl, submseteq_swap. Qed.
-  Lemma tctx_extract_hasty_here_copy E L p1 p2 ty ty' T :
-    p1 = p2 → Copy ty → subtype E L ty ty' →
-    tctx_extract_hasty E L p1 ty' ((p2 ◁ ty)::T) ((p2 ◁ ty)::T).
-  Proof.
-    intros -> ??. apply (tctx_incl_frame_r _ [_] [_;_]).
-    etrans; first by apply copy_tctx_incl, _.
-    by apply (tctx_incl_frame_r _ [_] [_]), subtype_tctx_incl.
-  Qed.
-  Lemma tctx_extract_hasty_here E L p1 p2 ty ty' T :
-    p1 = p2 → subtype E L ty ty' → tctx_extract_hasty E L p1 ty' ((p2 ◁ ty)::T) T.
-  Proof.
-    intros -> ?. by apply (tctx_incl_frame_r _ [_] [_]), subtype_tctx_incl.
-  Qed.
-  Lemma tctx_extract_hasty_here_eq E L p1 p2 ty T :
-    p1 = p2 → tctx_extract_hasty E L p1 ty ((p2 ◁ ty)::T) T.
-  Proof. intros ->. by apply tctx_extract_hasty_here. Qed.
+  Definition tctx_extract_hasty {As Bs A} E L p (ty : type A) (T : tctx As) (T' : tctx Bs) f : Prop :=
+    tctx_incl E L T ((p ◁ ty) +:: T') f.
 
-  Definition tctx_extract_blocked E L p κ ty T T' : Prop :=
-    tctx_incl E L T ((p ◁{κ} ty)::T').
-  Lemma tctx_extract_blocked_cons E L p κ ty T T' x :
-    tctx_extract_blocked E L p κ ty T T' →
-    tctx_extract_blocked E L p κ ty (x::T) (x::T').
+  Definition xprod_extract {As A B Bs} (f : xprod As → xprod (B ^:: Bs)) : xprod (A ^:: As) → xprod (B ^:: A ^:: Bs) :=
+    λ '(a -:: ass), let '(b -:: bss) := f ass in b -:: a -:: bss.
+
+  (* Lemma tctx_extract_hasty_further {As Bs A B} E L p (ty : type B) vπ (T : tctx As) (T' : tctx Bs) f (x : tctx_elt A) :
+    tctx_extract_hasty E L p ty vπ T T' f →
+    tctx_extract_hasty E L p ty vπ (x+::T) (x+::T') (xprod_extract f).
   Proof.
-    move=> /(tctx_incl_frame_l [x]) /= Hincl. rewrite /tctx_extract_blocked.
-    etrans; first done. apply contains_tctx_incl, submseteq_swap.
+    rewrite /tctx_extract_hasty.
+    intros.
+    eapply tctx_incl_transitive;
+      [eapply tcx_incl_cons, H| apply contains_tctx_incl].
+      
+    Unshelve.
+    constructor.
+  Qed. *)
+    
+  (* Lemma tctx_extract_hasty_here_copy {A B As} E L f p1 p2 (ty : type A) vπ (ty' : type B)  (T : tctx As) :
+    p1 = p2 → Copy ty → subtype E L f ty ty' →
+    tctx_extract_hasty E L p1 ty' (f ∘ vπ) ((p2 ◁ ty)+::T) ((p2 ◁ ty [{ vπ}])+::T) (λ p, (f p.1, p)).
+  Proof.
+    intros -> ??. apply (tctx_incl_frame_r _ +[_] +[_;_] (λ p, (f p.1, p))).
+    eapply tctx_incl_transitive; first by apply copy_tctx_incl, _.
+    by apply (tctx_incl_frame_r _ +[_] +[_]), (subtype_tctx_incl _ _ _ _ f).
   Qed.
-  Lemma tctx_extract_blocked_here E L p κ ty T :
-    tctx_extract_blocked E L p κ ty ((p ◁{κ} ty)::T) T.
-  Proof. intros. by apply (tctx_incl_frame_r _ [_] [_]). Qed.
 
-  Definition tctx_extract_ctx E L T T1 T2 : Prop :=
-    tctx_incl E L T1 (T++T2).
-  Lemma tctx_extract_ctx_nil E L T:
-    tctx_extract_ctx E L [] T T.
-  Proof. by unfold tctx_extract_ctx. Qed.
-  Lemma tctx_extract_ctx_hasty E L T T1 T2 T3 p ty:
-    tctx_extract_hasty E L p ty T1 T2 → tctx_extract_ctx E L T T2 T3 →
-    tctx_extract_ctx E L ((p ◁ ty)::T) T1 T3.
-  Proof. unfold tctx_extract_ctx, tctx_extract_hasty=>->->//. Qed.
-  Lemma tctx_extract_ctx_blocked E L T T1 T2 T3 p κ ty:
-    tctx_extract_blocked E L p κ ty T1 T2 → tctx_extract_ctx E L T T2 T3 →
-    tctx_extract_ctx E L ((p ◁{κ} ty)::T) T1 T3.
-  Proof. unfold tctx_extract_ctx, tctx_extract_blocked=>->->//. Qed.
+  Lemma tctx_extract_hasty_here {A B As} E L f p1 p2 (ty : type A) vπ (ty' : type B) (T : tctx As) :
+    p1 = p2 → subtype E L f ty ty' → tctx_extract_hasty E L p1 ty' (f ∘ vπ) ((p2 ◁ ty)+::T) T  (λ p, (f p.1, p.2)).
+  Proof.
+    intros -> ?. by apply (tctx_incl_frame_r _ +[_] +[_] (λ p, (f p.1, p.2))), (subtype_tctx_incl _ _ _ _ f).
+  Qed.
 
-  Lemma tctx_extract_ctx_incl E L T T' T0:
+  Lemma tctx_extract_hasty_here_eq {A As} E L p1 p2 (ty : type A) vπ (T : tctx As) :
+    p1 = p2 → tctx_extract_hasty E L p1 ty vπ ((p2 ◁ ty)+::T) T id.
+  Proof. intros ->. by eapply (tctx_extract_hasty_here _ _ id), subtype_refl. Qed. *)
+(* 
+  Definition tctx_extract_blocked {A As Bs} E L p κ (ty : type A) vπ (T : tctx As) (T' : tctx Bs) f : Prop :=
+    tctx_incl E L T ((p ◁{κ} ty)+::T') (λ A, vπ +:: f). *)
+
+  (* Lemma tctx_extract_blocked_cons {A B As Bs} E L p κ (ty : type B) vπ (T : tctx As) (T' : tctx Bs) (x : tctx_elt A) f :
+    tctx_extract_blocked E L p κ ty vπ T T' f →
+    tctx_extract_blocked E L p κ ty vπ (x+::T) (x+::T') (xprod_extract f).
+  Proof.
+    rewrite /tctx_extract_blocked.
+    intros.
+    eapply tctx_incl_transitive;
+      [eapply tcx_incl_cons, H| apply contains_tctx_incl].
+      
+    Unshelve.
+    constructor.
+  Qed. *)
+
+  (* Lemma tctx_extract_blocked_here {A As} E L p κ (ty : type A) vπ (T : tctx As) f:
+    tctx_extract_blocked E L p κ ty vπ ((p ◁{κ} ty)+::T) T f.
+  Proof. intros. apply (tctx_incl_frame_r _ +[_] +[_] id), tctx_incl_reflexive. Qed. *)
+
+  Definition tctx_extract_ctx {As Bs Cs} E L (T : tctx As) (T1 : tctx Bs) (T2 : tctx Cs) f : Prop :=
+    tctx_incl E L T1 (T h++T2) f.
+
+  Lemma tctx_extract_ctx_nil {As} E L (T : tctx As):
+    tctx_extract_ctx E L +[] T T id.
+  Proof. apply tctx_incl_reflexive. Qed.
+
+  Definition tctx_extract_ctx_hasty_trans {A As Bs Cs Ds} 
+    (f : (Π! (A ^:: Cs) → Prop) → Π! Bs → Prop ) 
+    (g : (Π! (As ^++ Ds) → Prop) → Π! Cs → Prop)
+  : (Π! ((A ^:: As) ^++ Ds) → Prop) → Π! Bs → Prop := 
+  λ post b, f (λ '(a -:: c),  g (λ ad, post (a -:: ad)) c) b.
+
+  Lemma tctx_extract_ctx_hasty {A As Bs Cs Ds} E L (T : tctx As) (T1 : tctx Bs) (T2 : tctx Cs) (T3 : tctx Ds) p (ty : type A) f g:
+    tctx_extract_hasty E L p ty T1 T2 f → tctx_extract_ctx E L T T2 T3 g →
+    tctx_extract_ctx E L ((p ◁ ty)+::T) T1 T3 (f ∘ trans_app (id : (Π! ^[A] → Prop) → _) g).
+  Proof. unfold tctx_extract_ctx, tctx_extract_hasty => ??.
+    eapply tctx_incl_transitive; [eassumption |  by eapply tcx_incl_cons]. 
+  Qed.
+  (*
+  Lemma tctx_extract_ctx_blocked {A As Bs Cs Ds} E L (T : tctx As) (T1 : tctx Bs) (T2 : tctx Cs) (T3 : tctx Ds) p κ (ty : type A) vπ:
+    tctx_extract_blocked E L p κ ty vπ T1 T2 → tctx_extract_ctx E L T T2 T3 →
+    tctx_extract_ctx E L ((p ◁{κ} ty)+::T) T1 T3.
+  Proof. unfold tctx_extract_ctx, tctx_extract_blocked => ?? //.
+    eapply tctx_incl_transitive, tcx_incl_cons; eassumption.
+  Qed.
+
+  Lemma tctx_extract_ctx_incl {As Bs Cs} E L (T : tctx As) (T' : tctx Bs) (T0 : tctx Cs):
     tctx_extract_ctx E L T' T T0 →
     tctx_incl E L T T'.
   Proof.
-    unfold tctx_extract_ctx=>->.
-      by apply contains_tctx_incl, submseteq_inserts_r.
-  Qed.
+    unfold tctx_extract_ctx=> ?.
+    eapply tctx_incl_transitive; first eassumption.
+    apply contains_tctx_incl, hsubmseteq_inserts_r, hpermutation_hsubmseteq, hpermutation_refl.
+  Qed. *)
 
   (* Unblocking a type context. *)
   (* TODO : That would be great if this could also remove all the
@@ -288,40 +386,40 @@ Section type_context.
      E.g., if [p ◁ &uniq{κ} ty] should be removed, because this is now
      useless. *)
 
-  Class UnblockTctx (κ : lft) (T1 T2 : tctx) : Prop :=
+  (* Class UnblockTctx (κ : lft) (A : Types) (T1 T2 : tctx A) : Prop :=
     unblock_tctx : ∀ tid, [†κ] -∗ tctx_interp tid T1 ={⊤}=∗ tctx_interp tid T2.
 
-  Global Instance unblock_tctx_nil κ : UnblockTctx κ [] [].
+  Global Instance unblock_tctx_nil κ : UnblockTctx κ _ +[] +[].
   Proof. by iIntros (tid) "_ $". Qed.
 
-  Global Instance unblock_tctx_cons_unblock T1 T2 p κ ty :
-    UnblockTctx κ T1 T2 →
-    UnblockTctx κ ((p ◁{κ} ty)::T1) ((p ◁ ty)::T2).
+  Global Instance unblock_tctx_cons_unblock A As (T1 T2 : tctx As) p κ (ty : type A) vπ:
+    UnblockTctx κ _ T1 T2 →
+    UnblockTctx κ _ ((p ◁{κ} ty) +:: T1) ((p ◁ ty) +:: T2).
   Proof.
     iIntros (H12 tid) "#H†". rewrite !tctx_interp_cons. iIntros "[H HT1]".
     iMod (H12 with "H† HT1") as "$". iDestruct "H" as (v) "[% H]".
     iMod ("H" with "H†") as (depth) "[??]". iExists v, depth. auto.
   Qed.
 
-  Global Instance unblock_tctx_cons κ T1 T2 x :
-    UnblockTctx κ T1 T2 → UnblockTctx κ (x::T1) (x::T2) | 100.
+  Global Instance unblock_tctx_cons κ A As (T1 T2 : tctx As) (x : tctx_elt A) :
+    UnblockTctx κ _ T1 T2 → UnblockTctx κ _ (x +:: T1) (x +:: T2) | 100.
   Proof.
     iIntros (H12 tid) "#H†". rewrite !tctx_interp_cons. iIntros "[$ HT1]".
     by iMod (H12 with "H† HT1") as "$".
-  Qed.
+  Qed.  *)
 End type_context.
 
-Global Hint Resolve tctx_extract_hasty_here_copy | 1 : lrust_typing.
+(* Global Hint Resolve tctx_extract_hasty_here_copy | 1 : lrust_typing.
 Global Hint Resolve tctx_extract_hasty_here | 20 : lrust_typing.
-Global Hint Resolve tctx_extract_hasty_further | 50 : lrust_typing.
-Global Hint Resolve tctx_extract_blocked_here tctx_extract_blocked_cons
-             tctx_extract_ctx_nil tctx_extract_ctx_hasty
-             tctx_extract_ctx_blocked tctx_extract_ctx_incl : lrust_typing.
-Global Hint Opaque tctx_extract_ctx tctx_extract_hasty tctx_extract_blocked
+Global Hint Resolve tctx_extract_hasty_further | 50 : lrust_typing. *)
+Global Hint Resolve (* tctx_extract_blocked_here tctx_extract_blocked_cons *)
+             tctx_extract_ctx_nil tctx_extract_ctx_hasty 
+             (* tctx_extract_ctx_blocked tctx_extract_ctx_incl *) : lrust_typing.
+Global Hint Opaque tctx_extract_ctx (* tctx_extract_hasty tctx_extract_blocked *)
             tctx_incl : lrust_typing.
 
 (* In general, we want reborrowing to be tried before subtyping, so
    that we get the extraction. However, in the case the types match
    exactly, we want to NOT use reborrowing. Therefore, we add
    [tctx_extract_hasty_here_eq] as a hint with a very low cost. *)
-Global Hint Resolve tctx_extract_hasty_here_eq | 2 : lrust_typing.
+(* Global Hint Resolve tctx_extract_hasty_here_eq | 2 : lrust_typing. *)
