theories/typing/bool.v
@@ -1,5 +1,9 @@
 From lrust.typing Require Export type.
-(* From lrust.typing Require Import programs. *)
+From lrust.typing Require Import programs.
+From lrust.util Require Import types.
+
+(* From lrust.util Require Import types. *)
+
 Set Default Proof Using "Type".
 
 Implicit Type b: bool.
@@ -13,32 +17,32 @@ Section bool.
 
   Global Instance bool_send: Send bool_ty. Proof. done. Qed.
 
-(*
-  Lemma type_bool_instr (b : Datatypes.bool) : typed_val #b bool.
+  Lemma type_bool_instr (b : Datatypes.bool) : typed_val #b bool_ty (λ post _, post -[b]).
   Proof.
-    iIntros (E L tid) "_ _ _ $ $ _". iMod persistent_time_receipt_0 as "#H0".
-    iApply wp_value. rewrite tctx_interp_singleton tctx_hasty_val' //.
-    iExists 0%nat. iFrame "H0". by destruct b.
+    iIntros (E L tid post ?) "_ _ _ $ $ _ ?". iMod persistent_time_receipt_0 as "#H0".
+    iApply wp_value. iExists +[const b]. iFrame. rewrite tctx_interp_singleton tctx_hasty_val' //. 
+    iExists 0%nat. iFrame "H0". eauto.
   Qed.
 
-  Lemma type_bool (b : Datatypes.bool) E L C T x e :
+  Lemma type_bool {As} (b : Datatypes.bool) E L C (T : tctx As) x e pre:
     Closed (x :b: []) e →
-    (∀ (v : val), typed_body E L C ((v ◁ bool) :: T) (subst' x v e)) -∗
-    typed_body E L C T (let: x := #b in e).
-  Proof. iIntros. iApply type_let; [apply type_bool_instr|solve_typing|done]. Qed.
-
-  Lemma type_if E L C T e1 e2 p:
-    p ◁ bool ∈ T →
-    typed_body E L C T e1 -∗ typed_body E L C T e2 -∗
-    typed_body E L C T (if: p then e1 else e2).
+    (∀ (v : val), typed_body E L C ((v ◁ bool_ty) +:: T) (subst' x v e) pre) -∗
+    typed_body E L C T (let: x := #b in e) (λ p, pre (b -:: p)).
+  Proof. iIntros. iApply type_let; [apply type_bool_instr|solve_typing|done|done]. Qed. 
+  
+  Lemma type_if {As} E L C (T : tctx As) e1 e2 p pre1 pre2:
+    p ◁ bool_ty ∈ T →
+    typed_body E L C T e1 pre1 -∗ typed_body E L C T e2 pre2 -∗
+    typed_body E L C T (if: p then e1 else e2) (λ a, pre1 a /\ pre2 a).
   Proof.
-    iIntros (Hp) "He1 He2". iIntros (tid) "#LFT #TIME #HE Htl HL HC HT".
-    iDestruct (big_sepL_elem_of _ _ _ Hp with "HT") as "#Hp".
+    iIntros (Hp) "He1 He2". iIntros (tid V) "#LFT #TIME #HE Htl HL HC HT Hv".
+    iDestruct (big_sepHLZip'_elem_of _ _ _ _ Hp with "HT") as (?) "#Hp".
     wp_bind p. iApply (wp_hasty with "Hp").
-    iIntros (depth [[| |[|[]|]]|]) "_ _ H1"; try done; wp_case.
-    - iApply ("He2" with "LFT TIME HE Htl HL HC HT").
+    iIntros (depth [[| |[|[]|]]|]) "_ _ H1"; try (iDestruct "H1" as ([|]) "[_ %]"; done); wp_case.
+    - iApply ("He2" with "LFT TIME HE Htl HL HC HT"). 
+      iApply (proph_obs_weaken with "Hv"). move => ? [? ?] //.
     - iApply ("He1" with "LFT TIME HE Htl HL HC HT").
+      iApply (proph_obs_weaken with "Hv"); move => ? [? ?] //.
   Qed.
-*)
 
 End bool.
